Sem.v
@@ -758,7 +758,7 @@ Qed.
 Lemma isrelease_dec : forall ad e,
   Decidable.decidable (is_release ad e).
 Proof.
-  unfold Decidable.decidable, not, is_acquire. intros ad' e; destruct e;
+  unfold Decidable.decidable, not, is_release. intros ad' e; destruct e;
   try solve [right; intros [F | F]; invc F];
   nat_eq_dec ad' ad; try solve [right; intros [F | F]; invc F; congruence];
   eauto.
